src/LibListZ.v
@@ -11,12 +11,9 @@ Require Export LibList LibNat.
 Require Import LibInt.
 Open Local Scope comp_scope.
 
-(** Set up specialized automation for this file *)
-
-Ltac auto_tilde ::= eauto with maths.
 
 (* ********************************************************************** *)
-(** * Z indices *)
+(** * List operations using indices in Z *)
 
 Section Zindices.
 Variables A : Type.
@@ -24,14 +21,38 @@ Implicit Types x : A.
 Implicit Types l : list A.
 Implicit Types i : int.
 
-Definition ZNth i l x := 
-  Nth (abs i) l x /\ 0 <= i.
+(** Set up specialized automation for this section *)
+Ltac auto_tilde ::= eauto with maths.
+
+
+(* ---------------------------------------------------------------------- *)
+(** * Definitions *)
+
+(** Functions *)
+
+Definition znth `{Inhab A} (i:int) (l:list A) :=
+  nth (abs i) l. 
+
+Definition zupdate (i:int) (v:A) (l:list A) :=
+  update (abs i) v l.
+
+Definition zmake (n:int) (v:A) :=
+  make (abs n) v.
+
+(** Predicates *)
 
 Definition ZInbound i l := 
   0 <= i /\ i < length l.
 
+Definition ZNth i l x := 
+  Nth (abs i) l x /\ 0 <= i.
+
 Definition ZUpdate i x l l' :=
   Update (abs i) x l l' /\ 0 <= i.
+
+
+(* ---------------------------------------------------------------------- *)
+(** * Znth *)
 
 Lemma ZNth_here : forall i x l,
   i = 0 -> ZNth i (x::l) x.
@@ -76,7 +97,7 @@ Proof using.
    math.
 Qed.
 
-Lemma ZNth_inboud : forall i l,
+Lemma ZNth_inbound : forall i l,
    ZInbound i l -> exists x, ZNth i l x.
 Proof using.
   introv [P U]. gen_eq n: (abs i). 
@@ -87,6 +108,10 @@ Proof using.
     forwards~: (@abs_spos i).
     exists x. split~. rewrite~ (@abs_spos i). constructor~.
 Qed.
+
+
+(* ---------------------------------------------------------------------- *)
+(** * ZInbound *)
 
 Lemma ZInbound_zero : forall x l,
   ZInbound 0 (x::l).
@@ -132,6 +157,10 @@ Lemma ZInbound_app_r_inv : forall i j l1 l2,
   ZInbound j (l1++l2) -> j = length l1 + i -> i >= 0 -> ZInbound i l2.
 Proof using. introv [P U] R H. rew_length in U. split~. Qed.
 
+
+(* ---------------------------------------------------------------------- *)
+(** * ZUpdate *)
+
 Lemma ZUpdate_here : forall x y l,
   ZUpdate 0 x (y::l) (x::l).
 Proof using. split~. apply Update_here. Qed.
@@ -165,8 +194,190 @@ Proof using. introv [U P]. apply~ Update_length. Qed.
 End Zindices.
 
 
-(* ********************************************************************** *)
-(** * Restore default automation *)
+(* ---------------------------------------------------------------------- *)
+(** ** Typeclasses read & update operations, binds and index predicates *)
 
-Ltac auto_tilde ::= auto_tilde_default.
+Definition read_impl `{Inhab A} (l:list A) (i:int) : A :=
+  znth i l.
+
+Definition update_impl A (l:list A) (i:int) (v:A) : array A :=
+  zupdate i v l.
+
+Definition binds_impl A (l:list A) (i:int) (v:A) := 
+  ZNth i l v.
+
+Definition index_impl A (l:list A) (i:int) =:
+  index (length l) i.
+
+Instance read_inst : forall `{Inhab A}, BagRead int A (list A).
+ constructor. rapply (@read_impl A H). Defined.
+Instance update_inst : forall A, BagUpdate int A (list A).
+  constructor. rapply (@update_impl A). Defined.
+Instance binds_inst : forall A, BagBinds int A (list A).
+  constructor. rapply (@binds_impl A). Defined.
+Instance index_inst : forall A, BagIndex (list A) int.
+  constructor. rapply (@index_impl A). Defined.
+
+Global Opaque array read_inst update_inst binds_inst index_inst.
+
+
+(* ---------------------------------------------------------------------- *)
+(** * Properties of zmake *)
+
+Lemma read_zmake : forall `{Inhab A} (i n:int) (v:A),
+  index n i -> (zmake n v)\(i) = v.
+Proof using.
+nth_make
+Qed.
+
+Lemma length_zmake : forall A n (v:A),
+  length (zmake n v) = n.
+Proof using.
+length_make
+Qed.
+
+
+(* ---------------------------------------------------------------------- *)
+(** * Properties of update *)
+
+Lemma length_update : forall (l:list A) (i:int) (v:A),
+  length (l\(i:=v)) = length l.
+Proof using.
+length_update
+Qed.
+
+Lemma read_update_eq : forall `{Inhab A} (l:list A) (i:int) (v:A),
+  index l i -> (l\(i:=v))\(i) = v.
+Proof using. 
+nth_update_eq
+Qed.
+
+Lemma read_update_neq : forall `{Inhab A} (l:list A) (i j:int) (v:A),
+  index l j -> (i <> j) -> (l\(i:=v))\(j) = l\(j).
+Proof using.
+nth_update_neq
+Qed.
+
+
+(* ---------------------------------------------------------------------- *)
+(** * Normalization tactics *)
+
+(** [rew_arr] is a light normalization tactic for array *)
+
+Hint Rewrite @read_update_eq : rew_arr.
+
+Tactic Notation "rew_arr" := 
+  autorewrite with rew_arr.
+Tactic Notation "rew_arr" "in" hyp(H) := 
+  autorewrite with rew_arr in H.
+Tactic Notation "rew_arr" "in" "*" := 
+  autorewrite with rew_arr in *.
+
+Tactic Notation "rew_arr" "~" :=
+  rew_arr; auto_tilde.
+Tactic Notation "rew_arr" "*" :=
+  rew_arr; auto_star.
+Tactic Notation "rew_arr" "~" "in" hyp(H) :=
+  rew_arr in H; auto_tilde.
+Tactic Notation "rew_arr" "*" "in" hyp(H) :=
+  rew_arr in H; auto_star.
+
+(** [rew_array] is a more aggressive normalization tactic for array *)
+
+Hint Rewrite @read_zmake @length_update @read_update_eq
+  @read_update_neq : rew_array.
+
+Tactic Notation "rew_array" := 
+  autorewrite with rew_array.
+Tactic Notation "rew_array" "in" hyp(H) := 
+  autorewrite with rew_array in H.
+Tactic Notation "rew_array" "in" "*" := 
+  autorewrite with rew_array in *.
+
+Tactic Notation "rew_array" "~" :=
+  rew_array; auto_tilde.
+Tactic Notation "rew_array" "*" :=
+  rew_array; auto_star.
+Tactic Notation "rew_array" "~" "in" hyp(H) :=
+  rew_array in H; auto_tilde.
+Tactic Notation "rew_array" "*" "in" hyp(H) :=
+  rew_array in H; auto_star.
+
+
+(* ---------------------------------------------------------------------- *)
+(** * Valid index predicate *)
+
+Section IndexProperties.
+Transparent Opaque array_index.
+
+Lemma index_def : forall A (l:list A) i,
+  index l i = index (length l) i.
+Proof using. auto. Qed. 
+
+Lemma index_length_eq : forall A (l:list A) i,
+  index (length l) i -> index l i.
+Proof using. introv H. rewrite* index_def. Qed.
+
+Lemma index_bounds : forall A (l:list A) i,
+  index l i = (0 <= i < length l).
+Proof using. auto. Qed. 
+
+Lemma index_prove : forall A (l:list A) i,
+  0 <= i < length l -> index l i.
+Proof using. intros. rewrite~ index_def. Qed.
+
+Lemma index_length : forall A (l:list A) n i,
+  index n i -> n = length l -> index l i.
+Proof using. intros. subst. rewrite~ index_def. Qed.
+
+Lemma index_update : forall `{Inhab A} (l:list A) i j (v:A),
+  index l i -> index (l\(j:=v)) i.
+Proof using. intros. rewrite index_def in *. rewrite length_update. Qed.
+
+Lemma index_zmake : forall `{Inhab A} n i (v:A),
+  index n i -> index (zmake n v) i.
+Proof using. intros.  Qed.
+
+End IndexProperties.
+
+
+(* ---------------------------------------------------------------------- *)
+(** * count *)
+
+(* TODO: complete definitions and proofs, which are used by CFML/Dijstra *)
+
+Require Import LibWf.
+
+(* TODO: implement a non-decidable version of count *)
+
+Parameter zcount : forall A (P:A->Prop) (l:list A), int.
+
+(* currently not used
+Parameter count_make : forall A (f:A->Prop) n v,
+  count f (make n v) = (If f v then n else 0).
+*)
+
+Parameter zcount_update : forall `{Inhab A} (P:A->Prop) (l:list A) (i:int) v,
+  index i l ->
+  zcount P (l\(i:=v)) = zcount f l
+    - (If P (l\(i)) then 1 else 0)
+    + (If P v then 1 else 0).
+
+Parameter zcount_bounds : forall `{Inhab A} (l:list A) (P:A->Prop),
+  0 <= zcount P l <= length l.
+
+(** The following lemma is used to argue that the update to a sequence,
+    when writing a value that satisfies [P] in place of one that did not
+    satisfy [P], decreases the total number of values that satisfying 
+    [P] in the sequence. *)
+
+Lemma zcount_upto : forall `{Inhab A} (P:A->Prop) (l:list A) (n i:int) (v:A),
+  ~ P (l\(i)) -> P v -> index i n -> length l <= n ->
+  upto n (zcount P (l\(i:=v))) (zcount P l).
+Proof using.
+  introv Ni Pv Hi Le. forwards K: (count_bounds (l\(i:=v)) P). split.
+  rewrite length_update in K. math.
+  lets M: (@count_update A _). rewrite M. clear M. 
+  do 2 (case_if; tryfalse). math.
+Qed.
 
